finished ftlr of cutdown version

theories/ftlr/interp_weakening.v
@@ -2,88 +2,29 @@ From cap_machine Require Export logrel.
 From iris.proofmode Require Import tactics.
 From iris.program_logic Require Import weakestpre adequacy lifting.
 From stdpp Require Import base.
-From cap_machine Require Import ftlr_base monotone region.
+From cap_machine Require Import ftlr_base region.
 From cap_machine Require Import addr_reg.
 
 Section fundamental.
   Context {Σ:gFunctors} {memg:memG Σ} {regg:regG Σ}
-          {stsg : STSG Addr region_type Σ} {heapg : heapG Σ}
-          `{MonRef: MonRefG (leibnizO _) CapR_rtc Σ} {nainv: logrel_na_invs Σ}
+          {nainv: logrel_na_invs Σ}
           `{MachineParameters}.
 
-  Notation STS := (leibnizO (STS_states * STS_rels)).
-  Notation STS_STD := (leibnizO (STS_std_states Addr region_type)).
-  Notation WORLD := (prodO STS_STD STS). 
-  Implicit Types W : WORLD.
-
-  Notation D := (WORLD -n> (leibnizO Word) -n> iProp Σ).
-  Notation R := (WORLD -n> (leibnizO Reg) -n> iProp Σ).
+  Notation D := ((leibnizO Word) -n> iProp Σ).
+  Notation R := ((leibnizO Reg) -n> iProp Σ).
   Implicit Types w : (leibnizO Word).
   Implicit Types interp : (D).
 
   Definition IH: iProp Σ :=
-    (□ ▷ (∀ (a7 : WORLD) (a8 : Reg) (a9 : Perm) (a10 : Locality) 
-           (a11 a12 a13 : Addr),
-            full_map a8
-                     -∗ (∀ r1 : RegName,
-                            ⌜r1 ≠ PC⌝
-                            → ((fixpoint interp1) a7)
-                                match a8 !! r1 with
-                                | Some w0 => w0
-                                | None => inl 0%Z
-                                end)
-                     -∗ registers_mapsto (<[PC:=inr (a9, a10, a11, a12, a13)]> a8)
-                     -∗ region a7
-                     -∗ sts_full_world a7
-                     -∗ na_own logrel_nais ⊤
-                     -∗ ⌜a9 = RX ∨ a9 = RWX ∨ a9 = RWLX ∧ a10 = Local⌝
-            → □ ([∗ list] a14 ∈ region_addrs a11 a12,
-                 ∃ p'0 : Perm,
-                   ⌜PermFlows a9 p'0⌝
-                      ∗ read_write_cond a14 p'0 interp
-                       ∧ ⌜if pwl a9
-                          then region_state_pwl a7 a14
-                          else region_state_nwl a7 a14 a10⌝) -∗ 
-                interp_conf a7))%I.
+    (□ ▷ (∀ a0 a1 a2 a3 a4,
+             full_map a0
+          -∗ (∀ r1 : RegName, ⌜r1 ≠ PC⌝ → (fixpoint interp1) (a0 !r! r1))
+          -∗ registers_mapsto (<[PC:=inr (a1, a2, a3, a4)]> a0)
+          -∗ na_own logrel_nais ⊤
+          -∗ ⌜a1 = RX ∨ a1 = RWX⌝
+             → □ (fixpoint interp1) (inr (a1, a2, a3, a4)) -∗ interp_conf))%I.
 
-  (* TODO: Move in monotone ? *)
-  Lemma region_state_nwl_future W W' l l' p a:
-    LocalityFlowsTo l' l ->
-    (if pwlU p then l = Local else True) ->
-    (@future_world Σ l' W W') -∗
-    ⌜if pwlU p then region_state_pwl W a else region_state_nwl W a l⌝ -∗
-    ⌜region_state_nwl W' a l'⌝.
-  Proof.
-    intros Hlflows Hloc. iIntros "Hfuture %".
-    destruct l'; simpl; iDestruct "Hfuture" as %Hf; iPureIntro.
-    - assert (l = Global) as -> by (destruct l; simpl in Hlflows; tauto).
-      destruct (pwlU p) eqn:HpwlU; try congruence.
-      eapply region_state_nwl_monotone_nl; eauto.
-    - destruct (pwlU p).
-      + subst l. left. eapply region_state_pwl_monotone; eauto.
-      + generalize (region_state_nwl_monotone _ _ _ _ Hf a0).
-        destruct l; auto.
-  Qed.
-
-  Lemma region_state_future W W' l l' p p' a:
-    PermFlowsTo p' p ->
-    LocalityFlowsTo l' l ->
-    (if pwlU p then l = Local else True) ->
-    (@future_world Σ l' W W') -∗
-    ⌜if pwlU p then region_state_pwl W a else region_state_nwl W a l⌝ -∗
-    ⌜if pwlU p' then region_state_pwl W' a else region_state_nwl W' a l'⌝.
-  Proof.
-    intros Hpflows Hlflows Hloc. iIntros "Hfuture %".
-    case_eq (pwlU p'); intros.
-    - assert (pwlU p = true) as Hpwl.
-      { destruct p, p'; simpl in H; try congruence; simpl in Hpflows; try tauto. }
-      rewrite Hpwl in a0, Hloc. subst l.
-      destruct l'; simpl in Hlflows; try tauto.
-      simpl; iDestruct "Hfuture" as "%"; iPureIntro.
-      eapply region_state_pwl_monotone; eauto.
-    - iApply (region_state_nwl_future with "Hfuture"); eauto.
-  Qed.
-
+ 
   (* TODO: Move somewhere ?*)
   Lemma PermFlowsToPermFlows p p':
     PermFlowsTo p p' <-> PermFlows p p'.
@@ -92,333 +33,61 @@ Section fundamental.
     destruct (Is_true_reflect (PermFlowsTo p p')); auto.
   Qed.
 
-  Lemma localityflowsto_futureworld l l' W W':
-    LocalityFlowsTo l' l ->
-    (@future_world Σ l' W W' -∗
-     @future_world Σ l W W').
-  Proof.
-    intros; destruct l, l'; auto.
-    rewrite /future_world; iIntros "%".
-    iPureIntro. eapply related_sts_pub_priv_world; auto.
-  Qed.
-
-  Lemma promote_perm_flows_monotone p p':
-    PermFlowsTo p p' ->
-    PermFlowsTo (promote_perm p) (promote_perm p').
-  Proof.
-    destruct p, p'; simpl; tauto.
-  Qed.
-
-  Lemma promote_perm_flows p:
-    PermFlowsTo p (promote_perm p).
-  Proof.
-    destruct p; simpl; tauto.
-  Qed.
-
-  Lemma promote_perm_pwl p:
-    pwl (promote_perm p) = pwlU p.
-  Proof.
-    destruct p; reflexivity.
-  Qed.
-
   Instance if_persistent (PROP: bi) (b: bool) (φ1 φ2: PROP) (H1: Persistent φ1) (H2: Persistent φ2):
     Persistent (if b then φ1 else φ2).
   Proof.
     destruct b; auto.
   Qed.
 
-  Lemma interp_weakening W p p' l l' b b' e e' a a'
-        (HU: if isU p then (a' <= a)%a else True):
+  Lemma interp_weakening p p' b b' e e' a a':
       p <> E ->
       (b <= b')%a ->
       (e' <= e)%a ->
       PermFlowsTo p' p ->
-      LocalityFlowsTo l' l ->
       IH -∗
-      (fixpoint interp1) W (inr (p, l, b, e, a)) -∗
-      (fixpoint interp1) W (inr (p', l', b', e', a')).
+      (fixpoint interp1) (inr (p, b, e, a)) -∗
+      (fixpoint interp1) (inr (p', b', e', a')).
   Proof.
-    intros HpnotE Hb He Hp Hl. iIntros "#IH HA".
-    rewrite !fixpoint_interp1_eq !interp1_eq.
-    destruct (perm_eq_dec p' O); auto.
-    destruct (perm_eq_dec p O).
-    { subst p; destruct p'; simpl in Hp; try tauto. }
-    destruct (perm_eq_dec p E); try congruence.
-    iDestruct "HA" as "[#A [% #C]]".
-    destruct (perm_eq_dec p' E).
-    { (* p' = E *) subst p'. iAlways.
-      assert (HisU: isU p = false).
-      { destruct p; simpl in Hp; simpl; auto; tauto. }
-      rewrite !HisU /enter_cond /interp_expr /=.
-      iIntros (r W') "#Hfuture". iNext.
-      iIntros "[[Hfull Hmap] [Hreg [Hregion [Hsts Hown]]]]".
-      iSplitR; auto. rewrite /interp_conf.
-      iApply ("IH" with "Hfull Hmap Hreg Hregion Hsts Hown"); eauto.
-      iAlways. simpl. destruct (Addr_le_dec b' e').
-      - rewrite (isWithin_region_addrs_decomposition b' e' b e); try solve_addr.
-        rewrite !big_sepL_app. iDestruct "A" as "[A1 [A2 A3]]".
-        iApply (big_sepL_impl with "A2"); auto. iAlways; iIntros (k x Hx) "Hw".
-        iDestruct "Hw" as (p'' Hflows) "[#X %]".
-        assert (Hflows': PermFlows RX p'').
-        { eapply PermFlows_trans; eauto.
-          destruct p; simpl in *; auto; try congruence; try tauto; reflexivity. }
-        iExists p''; iSplitR; eauto.
-        repeat iSplitR; auto.
-        iApply (region_state_nwl_future with "Hfuture"); eauto.
-      - rewrite (region_addrs_empty b' e'); auto. solve_addr. }
-    iSplit.
-    { destruct (isU p') eqn:HisU'.
-      { destruct (isU p) eqn:HisU.
-        - destruct l; destruct l'; simpl.
-          + destruct (Addr_le_dec b' e').
-            { rewrite (isWithin_region_addrs_decomposition b' e' b e); try solve_addr.
-              rewrite !big_sepL_app. iDestruct "A" as "[A1 [A2 A3]]".
-              iApply (big_sepL_impl with "A2"); auto. iAlways; iIntros (k x Hx) "Hw".
-              iDestruct "Hw" as (p'' Hflows) "[#X %]".
-              assert (Hpfl: PermFlows (promote_perm p') p'').
-              { eapply PermFlowsToPermFlows. eapply PermFlowsToTransitive; eauto. eapply promote_perm_flows_monotone; eauto. }
-              assert (Hpfl2: PermFlows p' p'').
-              { eapply PermFlows_trans; eauto. eapply PermFlowsToPermFlows.
-                eapply promote_perm_flows. }
-              iExists p''; iSplitR; auto.
-              repeat iSplit; auto.
-              case_eq (pwlU p'); intros.
-              + assert (pwlU p = true) as HP by (destruct p, p'; naive_solver).
-                rewrite HP in H1. iPureIntro. auto.
-              + iApply (region_state_nwl_future W W Global Global); eauto.
-                simpl. iPureIntro. eapply related_sts_priv_refl_world. }
-            { rewrite (region_addrs_empty b' e'); auto. solve_addr. }
-          + destruct (Addr_le_dec b' (min a' e')).
-            { rewrite (isWithin_region_addrs_decomposition b' (min a' e') b e). 2: solve_addr.
-              rewrite !big_sepL_app. iDestruct "A" as "[A1 [A2 A3]]".
-              iApply (big_sepL_impl with "A2"); auto. iAlways; iIntros (k x Hx) "Hw".
-              iDestruct "Hw" as (p'' Hflows) "[#X %]".
-              assert (Hpfl: PermFlows (promote_perm p') p'').
-              { eapply PermFlowsToPermFlows. eapply PermFlowsToTransitive; eauto. eapply promote_perm_flows_monotone; eauto. }
-              assert (Hpfl2: PermFlows p' p'').
-              { eapply PermFlows_trans; eauto. eapply PermFlowsToPermFlows.
-                eapply promote_perm_flows. }
-              iExists p''; iSplitR; auto.
-              repeat iSplit; auto.
-              case_eq (pwlU p'); intros.
-              * assert (pwlU p = true) as HP by (destruct p, p'; naive_solver).
-                rewrite HP in H1. iPureIntro. auto.
-              * iApply (region_state_nwl_future W W Global Local); eauto.
-                simpl. iPureIntro. eapply related_sts_pub_refl_world. }
-            { rewrite (region_addrs_empty b' (min a' e')); auto. solve_addr. }
-          + simpl in Hl. elim Hl.
-          + destruct (Addr_le_dec b' (min a' e')).
-            { rewrite (isWithin_region_addrs_decomposition b' (min a' e') b (min a e)). 2: solve_addr.
-              rewrite !big_sepL_app. iDestruct "A" as "[A1 [A2 A3]]".
-              iApply (big_sepL_impl with "A2"); auto. iAlways; iIntros (k x Hx) "Hw".
-              iDestruct "Hw" as (p'' Hflows) "[#X %]".
-              assert (Hpfl: PermFlows (promote_perm p') p'').
-              { eapply PermFlowsToPermFlows. eapply PermFlowsToTransitive; eauto. eapply promote_perm_flows_monotone; eauto. }
-              assert (Hpfl2: PermFlows p' p'').
-              { eapply PermFlows_trans; eauto. eapply PermFlowsToPermFlows.
-                eapply promote_perm_flows. }
-              iExists p''; iSplitR; auto.
-              repeat iSplit; auto.
-              case_eq (pwlU p'); intros.
-              * assert (pwlU p = true) as HP by (destruct p, p'; naive_solver).
-                rewrite HP in H1. iPureIntro. auto.
-              * iApply (region_state_nwl_future W W Local Local); eauto.
-                simpl; iPureIntro. eapply related_sts_pub_refl_world. }
-            { rewrite (region_addrs_empty b' (min a' e')); auto. solve_addr. }
-        - simpl. destruct l'; simpl.
-          { destruct (Addr_le_dec b' e').
-            + rewrite (isWithin_region_addrs_decomposition b' e' b e). 2: solve_addr.
-              rewrite !big_sepL_app. iDestruct "A" as "[A1 [A2 A3]]".
-              iApply (big_sepL_impl with "A2"); auto. iAlways; iIntros (k x Hx) "Hw".
-              iDestruct "Hw" as (p'' Hflows) "[#X %]".
-              assert (Hpfl: PermFlows (promote_perm p') p'').
-              { eapply PermFlowsToPermFlows. eapply PermFlowsToTransitive; eauto. eapply promote_perm_flows_monotone; eauto. }
-              assert (Hpfl2: PermFlows p' p'').
-              { eapply PermFlows_trans; eauto. eapply PermFlowsToPermFlows.
-                eapply promote_perm_flows. }
-              iExists p''; iSplitR; auto.
-              repeat iSplit; auto.
-              case_eq (pwlU p'); intros.
-              * assert (pwlU p = true) as HP by (destruct p, p'; naive_solver).
-                rewrite HP in H1. iPureIntro. auto.
-              * iApply (region_state_nwl_future W W l Global); eauto.
-                simpl; iPureIntro. eapply related_sts_priv_refl_world.
-            + rewrite (region_addrs_empty b' e'); auto. solve_addr. }
-          { destruct (Addr_le_dec b' (min a' e')).
-            + rewrite (isWithin_region_addrs_decomposition b' (min a' e') b e). 2: solve_addr.
-              rewrite !big_sepL_app. iDestruct "A" as "[A1 [A2 A3]]".
-              iApply (big_sepL_impl with "A2"); auto. iAlways; iIntros (k x Hx) "Hw".
-              iDestruct "Hw" as (p'' Hflows) "[#X %]".
-              assert (Hpfl: PermFlows (promote_perm p') p'').
-              { eapply PermFlowsToPermFlows. eapply PermFlowsToTransitive; eauto. eapply promote_perm_flows_monotone; eauto. }
-              assert (Hpfl2: PermFlows p' p'').
-              { eapply PermFlows_trans; eauto. eapply PermFlowsToPermFlows.
-                eapply promote_perm_flows. }
-              iExists p''; iSplitR; auto.
-              repeat iSplit; auto.
-              case_eq (pwlU p'); intros.
-              * assert (pwlU p = true) as HP by (destruct p, p'; naive_solver).
-                rewrite HP in H1. iPureIntro. auto.
-              * iApply (region_state_nwl_future W W l Local); eauto.
-                simpl; iPureIntro; eapply related_sts_pub_refl_world.
-            + rewrite (region_addrs_empty b' (min a' e')); auto. solve_addr. } }
-      assert (HisU: isU p = false).
-      { destruct p', p; simpl in *; try tauto; try congruence. }
-      rewrite !HisU. simpl.
-      destruct (Addr_le_dec b' e').
-      - rewrite (isWithin_region_addrs_decomposition b' e' b e); try solve_addr.
-        rewrite !big_sepL_app. iDestruct "A" as "[A1 [A2 A3]]".
-        iApply (big_sepL_impl with "A2"); auto. iAlways; iIntros (k x Hx) "Hw".
-        iDestruct "Hw" as (p'' Hflows) "[#X %]".
-        assert (Hpfl: PermFlows (promote_perm p') p'').
-        { eapply PermFlowsToPermFlows. eapply PermFlowsToTransitive; eauto. eapply promote_perm_flows_monotone; eauto. }
-        assert (Hpfl2: PermFlows p' p'').
-        { eapply PermFlows_trans; eauto. eapply PermFlowsToPermFlows.
-          eapply promote_perm_flows. }
-        iExists p''; iSplitR; auto.
-        repeat iSplit; auto.
-        case_eq (pwlU p'); intros.
-        + assert (pwlU p = true) as HP by (destruct p, p'; naive_solver).
-          rewrite HP in H1. iPureIntro. auto.
-        + iApply region_state_nwl_future; eauto.
-          destruct l'; iPureIntro.
-          * eapply related_sts_priv_refl_world.
-          * eapply related_sts_pub_refl_world.
-      - rewrite (region_addrs_empty b' e'); auto. solve_addr. }
-    iSplit.
-    { case_eq (pwlU p'); intros; auto.
-      assert (pwlU p = true) as HP by (destruct p, p'; naive_solver).
-      rewrite HP in H0; subst l. destruct l'; simpl in Hl; try tauto. auto. }
-    { case_eq (pwlU p'); intros; auto.
-      - assert (pwlU p = true) as HP by (destruct p, p'; naive_solver).
-        rewrite HP in H0; subst l. destruct l'; simpl in Hl; try tauto.
-        destruct (isU p') eqn:HisU'; auto. simpl.
-        destruct (isU p) eqn:HisU; simpl.
-        + destruct (Addr_le_dec (max b' a') e').
-          * rewrite HP. destruct (Addr_lt_dec (max b' a') (max b a)).
-            { destruct (Addr_le_dec (max b a) e').
-              - rewrite (isWithin_region_addrs_decomposition (max b a) e' (max b a) e). 2: solve_addr.
-                rewrite !big_sepL_app. iDestruct "C" as "[C1 [C2 C3]]".
-                rewrite (isWithin_region_addrs_decomposition (max b a) e' (max b' a') e'). 2: solve_addr.
-                rewrite !big_sepL_app. rewrite (region_addrs_empty e' e'); [simpl; iFrame "#"|solve_addr].
-                assert (Heq: min a e = max b a) by solve_addr. rewrite Heq.
-                rewrite (isWithin_region_addrs_decomposition (max b' a') (max b a) b (max b a)). 2: solve_addr.
-                rewrite !big_sepL_app. iDestruct "A" as "[A1 [A2 A3]]". iFrame "#". 
-                repeat iSplit;auto.
-                + iApply (big_sepL_impl with "A2"); auto.
-                  iAlways; iIntros (k x Hx) "Hw".
-                  iDestruct "Hw" as (p'' Hflows) "[#X %]".
-                  assert (Hpfl: PermFlows (promote_perm p') p'').
-                  { eapply PermFlowsToPermFlows. eapply PermFlowsToTransitive; eauto. eapply promote_perm_flows_monotone; eauto. }
-                  iExists _. iSplit;eauto. iFrame "#". iPureIntro. left; auto.
-                + iApply (big_sepL_impl with "C2"); auto.
-                  iAlways; iIntros (k x Hx) "Hw".
-                  iDestruct "Hw" as (p'' Hflows) "[#X %]".
-                  assert (Hpfl: PermFlows (promote_perm p') p'').
-                  { eapply PermFlowsToPermFlows. eapply PermFlowsToTransitive; eauto. eapply promote_perm_flows_monotone; eauto. }
-                  iExists _. iSplit;eauto. 
-              - rewrite (isWithin_region_addrs_decomposition (max b' a') e' b (min a e)). 2: solve_addr.
-                rewrite !big_sepL_app. iDestruct "A" as "[A1 [A2 A3]]".
-                iApply (big_sepL_impl with "A2"); auto.
-                iAlways; iIntros (k x Hx) "Hw".
-                iDestruct "Hw" as (p'' Hflows) "[#X %]".
-                assert (Hpfl: PermFlows (promote_perm p') p'').
-                { eapply PermFlowsToPermFlows. eapply PermFlowsToTransitive; eauto. eapply promote_perm_flows_monotone; eauto. }
-                iExists _. iSplit;eauto. 
-                iFrame "#". iPureIntro. left; auto. }
-            { rewrite (isWithin_region_addrs_decomposition (max b' a') e' (max b a) e). 2: solve_addr.
-              rewrite !big_sepL_app. iDestruct "C" as "[C1 [C2 C3]]".
-              iApply (big_sepL_impl with "C2"); auto.
-              iAlways; iIntros (k x Hx) "Hw".
-              iDestruct "Hw" as (p'' Hflows) "[#X %]".
-              assert (Hpfl: PermFlows (promote_perm p') p'').
-              { eapply PermFlowsToPermFlows. eapply PermFlowsToTransitive; eauto. eapply promote_perm_flows_monotone; eauto. }
-              iExists _. iSplit;eauto. 
-            }
-          * rewrite (region_addrs_empty (max b' a') e'); auto. solve_addr.
-        + destruct (Addr_le_dec (max b' a') e').
-          * rewrite HP. rewrite (isWithin_region_addrs_decomposition (max b' a') e' b e). 2: solve_addr.
-            rewrite !big_sepL_app. iDestruct "A" as "[A1 [A2 A3]]".
-            iApply (big_sepL_impl with "A2"); auto.
-            iAlways; iIntros (k x Hx) "Hw".
-            iDestruct "Hw" as (p'' Hflows) "[#X %]".
-            assert (Hpfl: PermFlows (promote_perm p') p'').
-            { eapply PermFlowsToPermFlows. eapply PermFlowsToTransitive; eauto. eapply promote_perm_flows_monotone; eauto. }
-            iExists _. iSplit;eauto. 
-            iFrame "#". iPureIntro. left; auto.
-          * rewrite (region_addrs_empty (max b' a') e'); auto. solve_addr.
-      - destruct (isU p') eqn:HisU'; simpl; auto.
-        destruct (isLocal l') eqn:Hl'; auto.
-        destruct (isU p && isLocal l) eqn:X.
-        + destruct (Addr_le_dec (max b' a') e').
-          * destruct (Addr_lt_dec (max b' a') (max b a)).
-            { destruct (Addr_le_dec (max b a) e').
-              - rewrite (isWithin_region_addrs_decomposition (max b a) e' (max b a) e). 2: solve_addr.
-                rewrite !big_sepL_app. iDestruct "C" as "[C1 [C2 C3]]".
-                rewrite (isWithin_region_addrs_decomposition (max b a) e' (max b' a') e'). 2: solve_addr.
-                rewrite !big_sepL_app. rewrite (region_addrs_empty e' e'); [simpl; iFrame "#"|solve_addr].
-                assert (Heq: min a e = max b a) by solve_addr. rewrite Heq.
-                rewrite (isWithin_region_addrs_decomposition (max b' a') (max b a) b (max b a)). 2: solve_addr.
-                rewrite !big_sepL_app. iDestruct "A" as "[A1 [A2 A3]]".
-                iSplitR.
-                + iApply (big_sepL_impl with "A2"); auto.
-                  iAlways; iIntros (k x Hx) "Hw".
-                  iDestruct "Hw" as (p'' Hflows) "[#X %]".
-                  assert (Hpfl: PermFlows (promote_perm p') p'').
-                  { eapply PermFlowsToPermFlows. eapply PermFlowsToTransitive; eauto. eapply promote_perm_flows_monotone; eauto. }
-                  iExists _. iSplit;eauto. 
-                  iFrame "#". iPureIntro. destruct (pwlU p).
-                  { left; auto. }
-                  { destruct l; simpl in H1; auto.
-                    - right; left; auto.
-                    - destruct H2; [left|right;left]; auto. }
-                + iSplitL; auto. iApply (big_sepL_impl with "C2"); auto.
-                  iAlways; iIntros (k x Hx) "Hw".
-                  iDestruct "Hw" as (p'' Hflows) "[#X %]".
-                  assert (Hpfl: PermFlows (promote_perm p') p'').
-                  { eapply PermFlowsToPermFlows. eapply PermFlowsToTransitive; eauto. eapply promote_perm_flows_monotone; eauto. }
-                  iExists _. iSplit;eauto. iFrame "X". 
-                  iPureIntro; 
-                  destruct p; simpl in H1; auto; destruct H2; rewrite /region_state_U; auto.
-              - rewrite (isWithin_region_addrs_decomposition (max b' a') e' b (min a e)). 2: solve_addr.
-                rewrite !big_sepL_app. iDestruct "A" as "[A1 [A2 A3]]".
-                iApply (big_sepL_impl with "A2"); auto.
-                iAlways; iIntros (k x Hx) "Hw".
-                iDestruct "Hw" as (p'' Hflows) "[#X %]".
-                assert (Hpfl: PermFlows (promote_perm p') p'').
-                { eapply PermFlowsToPermFlows. eapply PermFlowsToTransitive; eauto. eapply promote_perm_flows_monotone; eauto. }
-                iExists _. iSplit;eauto.
-                iFrame "#". iPureIntro. destruct (pwlU p).
-                + left; auto.
-                + destruct l; simpl in H1; auto.
-                  * right; left; auto.
-                  * destruct H2; [left|right;left]; auto. }
-            { rewrite (isWithin_region_addrs_decomposition (max b' a') e' (max b a) e). 2: solve_addr.
-              rewrite !big_sepL_app. iDestruct "C" as "[C1 [C2 C3]]". auto.
-              iApply (big_sepL_impl with "C2"); auto.
-              iAlways; iIntros (k x Hx) "Hw".
-              iDestruct "Hw" as (p'' Hflows) "[#X %]".
-              assert (Hpfl: PermFlows (promote_perm p') p'').
-              { eapply PermFlowsToPermFlows. eapply PermFlowsToTransitive; eauto. eapply promote_perm_flows_monotone; eauto. }
-              iExists _. iSplit;eauto. iFrame "#".
-              iPureIntro; 
-              destruct p; simpl in H2; auto; destruct H2; rewrite /region_state_U; auto. }
-          * rewrite (region_addrs_empty (max b' a') e'); auto. solve_addr.
-        + destruct (Addr_le_dec (max b' a') e').
-          * rewrite (isWithin_region_addrs_decomposition (max b' a') e' b e). 2: solve_addr.
-            rewrite !big_sepL_app. iDestruct "A" as "[A1 [A2 A3]]".
-            iApply (big_sepL_impl with "A2"); auto.
-            iAlways; iIntros (k x Hx) "Hw".
-            iDestruct "Hw" as (p'' Hflows) "[#X %]".
-            assert (Hpfl: PermFlows (promote_perm p') p'').
-            { eapply PermFlowsToPermFlows. eapply PermFlowsToTransitive; eauto. eapply promote_perm_flows_monotone; eauto. }
-            iExists _. iSplit;eauto.
-            iFrame "#". iPureIntro. destruct (pwlU p).
-            { left; auto. }
-            { destruct l; simpl in H2; auto.
-              - right; left; auto.
-              - destruct H2; [left|right;left]; auto. }
-          * rewrite (region_addrs_empty (max b' a') e'); auto. solve_addr. }
-  Qed.
+    intros HpnotE Hb He Hp. iIntros "#IH #HA".
+    destruct (decide (b' <= e')%a).
+    2: { rewrite !fixpoint_interp1_eq. destruct p'; try done; try (by iClear "HA"; rewrite /= !region_addrs_empty;[|solve_addr]).
+         iAlways. iIntros (r). iNext. iIntros "([Hfull Hreg] & Hregs & Hna)". iSplit;auto.
+         iApply ("IH" with "Hfull Hreg Hregs Hna"); auto. iAlways.
+         iClear "HA". by rewrite !fixpoint_interp1_eq /= !region_addrs_empty;[|solve_addr]. 
+    }  
+    destruct p'.
+    - rewrite !fixpoint_interp1_eq. done.
+    - rewrite !fixpoint_interp1_eq.
+      destruct p;inversion Hp;
+      (rewrite /= (isWithin_region_addrs_decomposition b' e' b e); [|solve_addr]);
+      rewrite !big_sepL_app; iDestruct "HA" as "[A1 [A2 A3]]";iFrame "#".
+      + iApply (big_sepL_mono with "A2").
+        iIntros (k y Hsome) "H". iDestruct "H" as (P) "(H1 & H2 & H3)". iExists P. iFrame. 
+      + iApply (big_sepL_mono with "A2").
+        iIntros (k y Hsome) "H". iDestruct "H" as (P) "(H1 & H2 & H3)". iExists P. iFrame.
+    - rewrite !fixpoint_interp1_eq.
+      destruct p;inversion Hp;
+      (rewrite /= (isWithin_region_addrs_decomposition b' e' b e); [|solve_addr]);
+      rewrite !big_sepL_app; iDestruct "HA" as "[A1 [A2 A3]]";iFrame "#".
+    - rewrite !fixpoint_interp1_eq.
+      destruct p;inversion Hp;
+      (rewrite /= (isWithin_region_addrs_decomposition b' e' b e); [|solve_addr]);
+      rewrite !big_sepL_app; iDestruct "HA" as "[A1 [A2 A3]]";iFrame "#".
+      iApply (big_sepL_mono with "A2").
+      iIntros (k y Hsome) "H". iDestruct "H" as (P) "(H1 & H2 & H3)". iExists P. iFrame.
+    - rewrite !fixpoint_interp1_eq. iAlways. iIntros (r). iNext. iIntros "([Hfull Hreg] & Hregs & Hna)". iSplit;auto.
+      iApply ("IH" with "Hfull Hreg Hregs Hna"); auto. iAlways.
+      destruct p; inversion Hp; try contradiction.
+      + rewrite /= (isWithin_region_addrs_decomposition b' e' b e); [|solve_addr].
+        rewrite !fixpoint_interp1_eq !big_sepL_app; iDestruct "HA" as "[A1 [A2 A3]]"; iFrame "#".
+      + rewrite /= (isWithin_region_addrs_decomposition b' e' b e); [|solve_addr].
+        rewrite !fixpoint_interp1_eq !big_sepL_app; iDestruct "HA" as "[A1 [A2 A3]]". 
+        iApply (big_sepL_mono with "A2").
+        iIntros (k y Hsome) "H". iDestruct "H" as (P) "(H1 & H2 & H3)". iExists P. iFrame. 
+    - rewrite !fixpoint_interp1_eq.
+      destruct p;inversion Hp;
+      (rewrite /= (isWithin_region_addrs_decomposition b' e' b e); [|solve_addr]);
+      rewrite !big_sepL_app; iDestruct "HA" as "[A1 [A2 A3]]";iFrame "#".
+  Qed. 
 
 End fundamental.
