theories/ftlr/IsPtr.v
@@ -7,27 +7,20 @@ From cap_machine.rules Require Import rules_IsPtr.
 
 Section fundamental.
   Context {Σ:gFunctors} {memg:memG Σ} {regg:regG Σ}
-          {stsg : STSG Addr region_type Σ} {heapg : heapG Σ}
-          `{MonRef: MonRefG (leibnizO _) CapR_rtc Σ} {nainv: logrel_na_invs Σ}
+          {nainv: logrel_na_invs Σ}
           `{MachineParameters}.
 
-  Notation STS := (leibnizO (STS_states * STS_rels)).
-  Notation STS_STD := (leibnizO (STS_std_states Addr region_type)).
-  Notation WORLD := (prodO STS_STD STS). 
-  Implicit Types W : WORLD.
-
-  Notation D := (WORLD -n> (leibnizO Word) -n> iProp Σ).
-  Notation R := (WORLD -n> (leibnizO Reg) -n> iProp Σ).
+  Notation D := ((leibnizO Word) -n> iProp Σ).
+  Notation R := ((leibnizO Reg) -n> iProp Σ).
   Implicit Types w : (leibnizO Word).
   Implicit Types interp : (D).
 
-  Lemma isptr_case (W : WORLD) (r : leibnizO Reg) (p p' : Perm)
-        (g : Locality) (b e a : Addr) (w : Word) (ρ : region_type) (dst r0 : RegName) :
-    ftlr_instr W r p p' g b e a w (IsPtr dst r0) ρ.
+  Lemma isptr_case (r : leibnizO Reg) (p : Perm)
+        (b e a : Addr) (w : Word) (dst r0 : RegName) (P:D) :
+    ftlr_instr r p b e a w (IsPtr dst r0) P.
   Proof.
-    intros Hp Hsome i Hbae Hfp Hpwl Hregion [Hnotrevoked Hnotstatic] HO Hi.
-    iIntros "#IH #Hinv #Hreg #Hinva Hmono #Hw Hsts Hown".
-    iIntros "Hr Hstate Ha HPC Hmap".
+    intros Hp Hsome i Hbae Hi.
+    iIntros "#IH #Hinv #Hinva #Hreg #[Hread Hwrite] Hown Ha HP Hcls HPC Hmap".
     rewrite delete_insert_delete.
     iDestruct ((big_sepM_delete _ _ PC) with "[HPC Hmap]") as "Hmap /=";
       [apply lookup_insert|rewrite delete_insert_delete;iFrame|]. simpl.
@@ -38,21 +31,19 @@ Section fundamental.
 
     iIntros "!>" (regs' retv). iDestruct 1 as (HSpec) "[Ha Hmap]".
     destruct HSpec; cycle 1.
-    { iApply wp_pure_step_later; auto. iNext.
+    { iApply wp_pure_step_later; auto. iMod ("Hcls" with "[HP Ha]");[iExists w;iFrame|iModIntro]. iNext.
       iApply wp_value; auto. iIntros; discriminate. }
     { incrementPC_inv; simplify_map_eq.
-      iApply wp_pure_step_later; auto. iNext.
+      iApply wp_pure_step_later; auto. iMod ("Hcls" with "[HP Ha]");[iExists w;iFrame|iModIntro]. iNext.
       assert (dst <> PC) as HdstPC. { intros ->. simplify_map_eq. }
       simplify_map_eq.
-      iDestruct (region_close with "[$Hstate $Hr $Ha $Hmono]") as "Hr"; eauto.
-      { destruct ρ;auto;[..|specialize (Hnotstatic g)];contradiction. }
-      iApply ("IH" $! _ (<[dst:= _]> _) with "[%] [] [Hmap] [$Hr] [$Hsts] [$Hown]");
+      iApply ("IH" $! (<[dst:= _]> _) with "[%] [] [Hmap] [$Hown]");
         try iClear "IH"; eauto.
       { cbn; intro. repeat (rewrite lookup_insert_is_Some'; right); eauto. }
       { iIntros (ri Hri). rewrite /RegLocate insert_commute // lookup_insert_ne //.
         destruct (decide (ri = dst)); simplify_map_eq.
         * repeat rewrite fixpoint_interp1_eq; auto.
-        * by iApply "Hreg". } }
+        * by iApply "Hreg". } rewrite !fixpoint_interp1_eq /=. destruct Hp as [-> | ->];iFrame "Hinv". }
   Qed.
 
 End fundamental.
