theories/ftlr/Lea.v
@@ -2,33 +2,25 @@ From cap_machine Require Export logrel.
 From iris.proofmode Require Import tactics.
 From iris.program_logic Require Import weakestpre adequacy lifting.
 From stdpp Require Import base.
-From cap_machine Require Import ftlr_base monotone.
+From cap_machine Require Import ftlr_base.
 From cap_machine Require Import rules_base interp_weakening.
 From cap_machine.rules Require Import rules_Lea.
 
 Section fundamental.
   Context {Σ:gFunctors} {memg:memG Σ} {regg:regG Σ}
-          {stsg : STSG Addr region_type Σ} {heapg : heapG Σ}
-          `{MonRef: MonRefG (leibnizO _) CapR_rtc Σ} {nainv: logrel_na_invs Σ}
+          {nainv: logrel_na_invs Σ}
           `{MachineParameters}.
-
-  Notation STS := (leibnizO (STS_states * STS_rels)).
-  Notation STS_STD := (leibnizO (STS_std_states Addr region_type)).
-  Notation WORLD := (prodO STS_STD STS). 
-  Implicit Types W : WORLD.
-
-  Notation D := (WORLD -n> (leibnizO Word) -n> iProp Σ).
-  Notation R := (WORLD -n> (leibnizO Reg) -n> iProp Σ).
+  Notation D := ((leibnizO Word) -n> iProp Σ).
+  Notation R := ((leibnizO Reg) -n> iProp Σ).
   Implicit Types w : (leibnizO Word).
   Implicit Types interp : (D).
 
-  Lemma lea_case (W : WORLD) (r : leibnizO Reg) (p p' : Perm)
-        (g : Locality) (b e a : Addr) (w : Word) (ρ : region_type) (dst : RegName) (r0 : Z + RegName):
-    ftlr_instr W r p p' g b e a w (Lea dst r0) ρ.
+  Lemma lea_case (r : leibnizO Reg) (p : Perm)
+        (b e a : Addr) (w : Word) (dst : RegName) (r0 : Z + RegName) (P:D):
+    ftlr_instr r p b e a w (Lea dst r0) P.
   Proof.
-    intros Hp Hsome i Hbae Hfp Hpwl Hregion [Hnotrevoked Hnotstatic] HO Hi.
-    iIntros "#IH #Hinv #Hreg #Hinva Hmono #Hw Hsts Hown".
-    iIntros "Hr Hstate Ha HPC Hmap".
+    intros Hp Hsome i Hbae Hi.
+    iIntros "#IH #Hinv #Hinva #Hreg #[Hread Hwrite] Hown Ha HP Hcls HPC Hmap".
     rewrite delete_insert_delete.
     iDestruct ((big_sepM_delete _ _ PC) with "[HPC Hmap]") as "Hmap /=";
       [apply lookup_insert|rewrite delete_insert_delete;iFrame|]. simpl.
@@ -38,16 +30,16 @@ Section fundamental.
       apply elem_of_gmap_dom. apply lookup_insert_is_Some'; eauto. }
 
     iIntros "!>" (regs' retv). iDestruct 1 as (HSpec) "[Ha Hmap]".
-    destruct HSpec as [ * Hdst ? Hz Hoffset HUa HincrPC |].
-    { apply incrementPC_Some_inv in HincrPC as (p''&g''&b''&e''&a''& ? & HPC & Z & Hregs').
+    destruct HSpec as [ * Hdst ? Hz Hoffset HincrPC |].
+    { apply incrementPC_Some_inv in HincrPC as (p''&b''&e''&a''& ? & HPC & Z & Hregs').
 
-      assert (p'' = p ∧ g'' = g ∧ b'' = b ∧ e'' = e) as (-> & -> & -> & ->).
+      assert (p'' = p ∧ b'' = b ∧ e'' = e) as (-> & -> & ->).
       { destruct (decide (PC = dst)); simplify_map_eq; auto. }
 
-      iApply wp_pure_step_later; auto. iNext.
-      iDestruct (region_close with "[$Hstate $Hr $Ha $Hmono]") as "Hr"; eauto.
-      { destruct ρ;auto;[..|specialize (Hnotstatic g1)];contradiction. }
-      iApply ("IH" $! _ regs' with "[%] [] [Hmap] [$Hr] [$Hsts] [$Hown]").
+      iApply wp_pure_step_later; auto.
+      iMod ("Hcls" with "[HP Ha]");[iExists w;iFrame|iModIntro]. 
+      iNext.
+      iApply ("IH" $! regs' with "[%] [] [Hmap] [$Hown]").
       { cbn. intros. subst regs'. by repeat (apply lookup_insert_is_Some'; right). }
       { iIntros (ri Hri). subst regs'.
         erewrite locate_ne_reg; [ | | reflexivity]; auto.
@@ -55,16 +47,15 @@ Section fundamental.
         { subst ri. unshelve iSpecialize ("Hreg" $! dst _); eauto.
           erewrite locate_eq_reg; [ | reflexivity]; auto. simplify_map_eq.
           rewrite /RegLocate Hdst. iApply interp_weakening; eauto; try solve_addr.
-          - destruct p0; simpl; auto.
-          - eapply PermFlowsToReflexive.
-          - destruct g0; auto. }
+          destruct p0; simpl; auto. } 
         { repeat (erewrite locate_ne_reg; [ | | reflexivity]; auto).
           iApply "Hreg"; auto. } }
       { subst regs'. rewrite insert_insert. iApply "Hmap". }
       { iPureIntro. tauto. }
-      eauto. }
-    { iApply wp_pure_step_later; auto. iNext.
-      iApply wp_value; auto. iIntros; discriminate. }
+      iAlways. rewrite !fixpoint_interp1_eq /=. destruct Hp as [-> | ->];iFrame "Hinv". }
+    { iApply wp_pure_step_later; auto.
+      iMod ("Hcls" with "[HP Ha]");[iExists w;iFrame|iModIntro]. 
+      iApply wp_value; auto. iNext. iIntros; discriminate. }
   Qed.
 
 End fundamental.
