theories/ftlr/Restrict.v
@@ -2,68 +2,36 @@ From cap_machine Require Export logrel.
 From iris.proofmode Require Import tactics.
 From iris.program_logic Require Import weakestpre adequacy lifting.
 From stdpp Require Import base.
-From cap_machine Require Import ftlr_base monotone interp_weakening.
+From cap_machine Require Import ftlr_base interp_weakening.
 From cap_machine.rules Require Import rules_base rules_Restrict.
 
 Section fundamental.
   Context {Σ:gFunctors} {memg:memG Σ} {regg:regG Σ}
-          {stsg : STSG Addr region_type Σ} {heapg : heapG Σ}
-          `{MonRef: MonRefG (leibnizO _) CapR_rtc Σ} {nainv: logrel_na_invs Σ}
+          {nainv: logrel_na_invs Σ}
           `{MachineParameters}.
-
-  Notation STS := (leibnizO (STS_states * STS_rels)).
-  Notation STS_STD := (leibnizO (STS_std_states Addr region_type)).
-  Notation WORLD := (prodO STS_STD STS). 
-  Implicit Types W : WORLD.
-
-  Notation D := (WORLD -n> (leibnizO Word) -n> iProp Σ).
-  Notation R := (WORLD -n> (leibnizO Reg) -n> iProp Σ).
+  
+  Notation D := ((leibnizO Word) -n> iProp Σ).
+  Notation R := ((leibnizO Reg) -n> iProp Σ).
   Implicit Types w : (leibnizO Word).
   Implicit Types interp : (D).
 
-  Lemma locality_eq_dec:
-    forall (l1 l2: Locality), {l1 = l2} + {l1 <> l2}.
-  Proof.
-    destruct l1, l2; auto.
-  Qed.
-
-  Lemma PermPairFlows_interp_preserved W p p' l l' b e a :
+  Lemma PermPairFlows_interp_preserved p p' b e a :
     p <> E ->
-    PermPairFlowsTo (p', l') (p, l) = true →
-    □ ▷ (∀ (a7 : WORLD) (a8 : Reg) (a9 : Perm) (a10 : Locality) 
-           (a11 a12 a13 : Addr),
-            full_map a8
-            -∗ (∀ r1 : RegName,
-                   ⌜r1 ≠ PC⌝
-                   → ((fixpoint interp1) a7)
-                       match a8 !! r1 with
-                       | Some w0 => w0
-                       | None => inl 0%Z
-                       end)
-            -∗ registers_mapsto (<[PC:=inr (a9, a10, a11, a12, a13)]> a8)
-            -∗ region a7
-            -∗ sts_full_world a7
-            -∗ na_own logrel_nais ⊤
-            -∗ ⌜a9 = RX ∨ a9 = RWX ∨ a9 = RWLX ∧ a10 = Local⌝
-            → □ ([∗ list] a14 ∈ region_addrs a11 a12,
-                 ∃ p'0 : Perm,
-                    ⌜PermFlows a9 p'0⌝ ∗
-                       read_write_cond a14 p'0 interp
-                       ∧ ⌜if pwl a9
-                          then region_state_pwl a7 a14
-                          else region_state_nwl a7 a14 a10⌝) -∗ 
-                interp_conf a7) -∗
-    (fixpoint interp1) W (inr (p, l, b, e, a)) -∗
-    (fixpoint interp1) W (inr (p', l', b, e, a)).
+    PermFlowsTo p' p = true →
+    (□ ▷ (∀ a0 a1 a2 a3 a4,
+             full_map a0
+          -∗ (∀ r1 : RegName, ⌜r1 ≠ PC⌝ → (fixpoint interp1) (a0 !r! r1))
+          -∗ registers_mapsto (<[PC:=inr (a1, a2, a3, a4)]> a0)
+          -∗ na_own logrel_nais ⊤
+          -∗ ⌜a1 = RX ∨ a1 = RWX⌝
+             → □ (fixpoint interp1) (inr (a1, a2, a3, a4)) -∗ interp_conf)) -∗
+    (fixpoint interp1) (inr (p, b, e, a)) -∗
+    (fixpoint interp1) (inr (p', b, e, a)).
   Proof.
     intros HpnotE Hp. iIntros "#IH HA".
-    destruct (andb_true_eq _ _ ltac:(symmetry in Hp; exact Hp)) as [HH1 HH2].
-    simpl in HH1, HH2. iApply (interp_weakening with "IH HA"); eauto; try solve_addr.
-    - destruct (isU p); solve_addr.
-    -  rewrite <- HH1. auto.
-    - rewrite <- HH2. auto.
+    iApply (interp_weakening with "IH HA"); eauto; try solve_addr.
   Qed.
-
+  
   Lemma match_perm_with_E_rewrite:
     forall (A: Type) p (a1 a2: A),
       match p with
@@ -74,13 +42,12 @@ Section fundamental.
     intros. destruct (perm_eq_dec p E); destruct p; auto; congruence.
   Qed.
 
-  Lemma restrict_case (W : WORLD) (r : leibnizO Reg) (p p' : Perm)
-        (g : Locality) (b e a : Addr) (w : Word) (ρ : region_type) (dst : RegName) (r0 : Z + RegName):
-    ftlr_instr W r p p' g b e a w (Restrict dst r0) ρ.
+  Lemma restrict_case (r : leibnizO Reg) (p : Perm)
+        (b e a : Addr) (w : Word) (dst : RegName) (r0 : Z + RegName) (P:D):
+    ftlr_instr r p b e a w (Restrict dst r0) P.
   Proof.
-    intros Hp Hsome i Hbae Hfp Hpwl Hregion [Hnotrevoked Hnotstatic] HO Hi.
-    iIntros "#IH #Hinv #Hreg #Hinva Hmono #Hw Hsts Hown".
-    iIntros "Hr Hstate Ha HPC Hmap".
+    intros Hp Hsome i Hbae Hi.
+    iIntros "#IH #Hinv #Hinva #Hreg #[Hread Hwrite] Hown Ha HP Hcls HPC Hmap".
     rewrite delete_insert_delete.
     iDestruct ((big_sepM_delete _ _ PC) with "[HPC Hmap]") as "Hmap /=";
       [apply lookup_insert|rewrite delete_insert_delete;iFrame|]. simpl.
@@ -91,13 +58,16 @@ Section fundamental.
 
     iIntros "!>" (regs' retv). iDestruct 1 as (HSpec) "[Ha Hmap]".
     destruct HSpec; cycle 1.
-    { iApply wp_pure_step_later; auto. iNext.
+    { iApply wp_pure_step_later; auto.
+      iMod ("Hcls" with "[HP Ha]");[iExists w;iFrame|iModIntro]. 
+      iNext.
       iApply wp_value; auto. iIntros; discriminate. }
     { match goal with
-      | H: incrementPC _ = Some _ |- _ => apply incrementPC_Some_inv in H as (p''&g''&b''&e''&a''& ? & HPC & Z & Hregs')
+      | H: incrementPC _ = Some _ |- _ => apply incrementPC_Some_inv in H as (p''&b''&e''&a''& ? & HPC & Z & Hregs')
       end. simplify_map_eq.
-      iApply wp_pure_step_later; auto. iNext.
-
+      iApply wp_pure_step_later; auto.
+      iMod ("Hcls" with "[HP Ha]");[iExists w;iFrame|iModIntro]. 
+      iNext. 
       assert (HPCr0: match r0 with inl _ => True | inr r0 => PC <> r0 end).
       { destruct r0; auto.
         intro; subst r0. simplify_map_eq. }
@@ -107,49 +77,36 @@ Section fundamental.
         repeat rewrite insert_insert in HPC.
         rewrite lookup_insert in HPC. inv HPC.
         rewrite lookup_insert in H0. inv H0.
-        rewrite H5 in H3. iDestruct (region_close with "[$Hstate $Hr $Ha $Hmono]") as "Hr"; eauto.
-        { destruct ρ;auto;[..|specialize (Hnotstatic g)];contradiction. }
-        destruct (PermFlowsTo RX p'') eqn:Hpft.
-        { assert (Hpg: p'' = RX ∨ p'' = RWX ∨ p'' = RWLX ∧ g'' = Local).
-          { destruct p''; simpl in Hpft; eauto; try discriminate.
-            destruct (andb_true_eq _ _ ltac:(naive_solver)).
-            simpl in H3, H4. destruct p0; simpl in H3; try discriminate.
-            destruct Hp as [Hp | [Hp | [Hp Hg] ] ]; try discriminate.
-            subst g0; destruct g''; simpl in H4; auto; discriminate. }
-          rewrite H5. iApply ("IH" $! _ r with "[%] [] [Hmap] [$Hr] [$Hsts] [$Hown]"); try iClear "IH"; eauto.
-          iAlways. iApply (big_sepL_mono with "Hinv"); simpl; intros.
-          iIntros "H". iDestruct "H" as (? ?) "[H %]". iExists H4. iSplitR; auto.
-          { destruct (andb_true_eq _ _ ltac:(naive_solver)).
-            iPureIntro. eapply PermFlows_trans with p0; auto. naive_solver. }
-          iSplitL;auto. 
-          iPureIntro. 
-          destruct (andb_true_eq _ _ ltac:(naive_solver)); simpl in *.
-          destruct (locality_eq_dec g'' g0).
-          * subst g0. destruct Hp as [Hp | [ Hp | [Hp Hl] ] ]; destruct Hpg as [Hp' | [ Hp' | [Hp' Hg' ] ] ]; subst; simpl in *; simpl; try congruence; auto.
-          * destruct g''; destruct g0; simpl in *; try congruence.
-            destruct Hp as [Hp | [ Hp | [Hp Hl] ] ]; destruct Hpg as [Hp' | [ Hp' | [Hp' Hg' ] ] ]; subst; simpl in *; simpl; try congruence; auto. }
+
+        destruct (PermFlowsTo RX (decodePerm n)) eqn:Hpft.
+        { assert (Hpg: (decodePerm n) = RX ∨ (decodePerm n) = RWX).
+          { destruct (decodePerm n); simpl in Hpft; eauto; try discriminate. }
+          iApply ("IH" $! r with "[%] [] [Hmap] [$Hown]");auto. 
+          iAlways. rewrite !fixpoint_interp1_eq /=.
+          destruct Hpg as [Heq | Heq];destruct Hp as [Heq' | Heq'];rewrite Heq Heq';try iFrame "Hinv".
+          - iApply (big_sepL_mono with "Hinv").
+            iIntros (k y _) "H". iDestruct "H" as (P') "(H1 & H2 & H3)". iExists P'. iFrame. 
+          - rewrite Heq Heq' in H3. inversion H3. 
+        }
         { iApply (wp_bind (fill [SeqCtx])).
           iDestruct ((big_sepM_delete _ _ PC) with "Hmap") as "[HPC Hmap]"; [apply lookup_insert|].
-         rewrite H5.
-          iApply (wp_notCorrectPC with "HPC"); [eapply not_isCorrectPC_perm; destruct p''; simpl in Hpft; eauto; discriminate|].
+          iApply (wp_notCorrectPC with "HPC"); [eapply not_isCorrectPC_perm; destruct (decodePerm n); simpl in Hpft; eauto; discriminate|].
           iNext. iIntros "HPC /=".
           iApply wp_pure_step_later; auto.
           iApply wp_value.
           iNext. iIntros. discriminate. } }
-
+      
       simplify_map_eq.
-      iDestruct (region_close with "[$Hstate $Hr $Ha $Hmono]") as "Hr"; eauto.
-      { destruct ρ;auto;[..|specialize (Hnotstatic g)];contradiction. }
-      iApply ("IH" $! _ (<[dst:=_]> _) with "[%] [] [Hmap] [$Hr] [$Hsts] [$Hown]"); eauto.
+      iApply ("IH" $! (<[dst:=_]> _) with "[%] [] [Hmap] [$Hown]"); eauto.
       - intros; simpl. repeat (rewrite lookup_insert_is_Some'; right); eauto.
       - iIntros (ri Hri). rewrite /RegLocate.
         destruct (decide (ri = dst)).
         + subst ri. rewrite lookup_insert.
-          destruct (decodePermPair n) as (p1 & g1).
           iDestruct ("Hreg" $! dst Hri) as "Hdst".
           rewrite H0. iApply PermPairFlows_interp_preserved; eauto.
         + repeat rewrite lookup_insert_ne; auto.
-          iApply "Hreg"; auto. }
+          iApply "Hreg"; auto.
+      - iAlways. rewrite !fixpoint_interp1_eq /=. destruct Hp as [-> | ->];iFrame "Hinv". }
   Qed.
 
 End fundamental.
